src/program_proof/mpaxos/applyasfollower_proof.v
@@ -1,0 +1,137 @@
+From Perennial.program_proof Require Import grove_prelude.
+From Goose.github_com.mit_pdos.gokv Require mpaxos.
+From Perennial.program_proof.grove_shared Require Import urpc_proof urpc_spec.
+From Perennial.goose_lang.lib Require Import waitgroup.
+From iris.base_logic Require Export lib.ghost_var mono_nat.
+From iris.algebra Require Import dfrac_agree mono_list.
+From Perennial.goose_lang Require Import crash_borrow.
+From Perennial.program_proof Require Import marshal_stateless_proof.
+From Perennial.program_proof.mpaxos Require Export definitions.
+
+Section applyasfollower_proof.
+
+Context `{!heapGS Σ}.
+Context {mp_record:MPRecord}.
+Notation OpType := (mp_OpType mp_record).
+Notation has_op_encoding := (mp_has_op_encoding mp_record).
+Notation next_state := (mp_next_state mp_record).
+Notation compute_reply := (mp_compute_reply mp_record).
+Notation is_Server := (is_Server (mp_record:=mp_record)).
+Notation applyAsFollower_core_spec := (applyAsFollower_core_spec).
+Notation is_singleClerk := (is_singleClerk (mp_record:=mp_record)).
+
+Context (conf:list mp_server_names).
+Context `{!mpG Σ}.
+
+Lemma wp_singleClerk__applyAsFollower ck γ γsrv σ Q args_ptr args reply_ptr init_reply :
+  {{{
+        "#His_ck" ∷ is_singleClerk conf ck γ γsrv ∗
+        "Hargs" ∷ applyAsFollowerArgs.own args_ptr args ∗
+        "Hreply" ∷ applyAsFollowerReply.own reply_ptr init_reply 1 ∗
+
+        "%Hσ_index" ∷ ⌜length σ = (int.nat args.(applyAsFollowerArgs.nextIndex) + 1)%nat⌝ ∗
+        "%Hghost_op_σ" ∷ ⌜last σ = Some (args.(applyAsFollowerArgs.state), Q)⌝ ∗
+        "%Hno_overflow" ∷ ⌜int.nat args.(applyAsFollowerArgs.nextIndex) < int.nat (word.add args.(applyAsFollowerArgs.nextIndex) 1)⌝ ∗
+        "#Hprop_lb" ∷ is_proposal_lb γ args.(applyAsFollowerArgs.epoch) σ ∗
+        "#Hprop_facts" ∷ is_proposal_facts conf γ args.(applyAsFollowerArgs.epoch) σ
+  }}}
+    singleClerk__applyAsFollower #ck #args_ptr #reply_ptr
+  {{{
+        reply, RET #(); applyAsFollowerReply.own reply_ptr reply 1 ∗
+                                                 □if (decide (reply.(applyAsFollowerReply.err) = (U64 0))) then
+                                                   is_accepted_lb γsrv args.(applyAsFollowerArgs.epoch) σ
+                                                 else
+                                                   True
+  }}}.
+Proof.
+Admitted.
+
+Lemma wp_Server__applyAsFollower (s:loc) (args_ptr reply_ptr:loc) γ γsrv args init_reply σ Q Φ Ψ :
+  is_Server conf s γ γsrv -∗
+  applyAsFollowerArgs.own args_ptr args -∗
+  applyAsFollowerReply.own reply_ptr init_reply 1 -∗
+  (∀ reply, Ψ reply -∗ applyAsFollowerReply.own reply_ptr reply 1 -∗ Φ #()) -∗
+  applyAsFollower_core_spec conf γ γsrv args σ Q Ψ -∗
+  WP mpaxos.Server__applyAsFollower #s #args_ptr #reply_ptr {{ Φ }}
+.
+Proof.
+  iIntros "#HisSrv Hpre Hreply HΦ HΨ".
+  iNamed "Hpre".
+  iNamed "HisSrv".
+  wp_call.
+  wp_loadField.
+  wp_apply (acquire_spec with "HmuInv").
+  iIntros "[Hlocked Hown]".
+  iNamed "Hown".
+  wp_pures.
+  wp_loadField.
+  wp_loadField.
+  wp_pures.
+  wp_if_destruct.
+  { (* case: s.epoch ≤ args.epoch *)
+    wp_loadField.
+    wp_loadField.
+    wp_pures.
+    wp_if_destruct.
+    { (* case: s.acceptedEpoch = args.epoch *)
+      wp_loadField.
+      wp_loadField.
+      wp_if_destruct.
+      { (* case: s.nextIndex == len(s.log) ≤ args.nextIndex *)
+        wp_loadField.
+        wp_storeField.
+        wp_loadField.
+        wp_storeField.
+        wp_storeField.
+        wp_loadField.
+        admit. (* TODO: use protocol lemma *)
+      }
+      { (* case: args.nextIndex < s.nextIndex len(s.log) *)
+        assert (int.Z (length st.(mp_log)) > int.Z args.(applyAsFollowerArgs.nextIndex))%Z as Hineq.
+        { word. }
+        wp_storeField.
+        wp_loadField.
+        admit. (* TODO: use protocol lemma *)
+      }
+    }
+    { (* case acceptedEpoch ≠ args.epoch, which implies
+         acceptedEpoch < args.epoch
+       *)
+      wp_loadField.
+      wp_storeField.
+      wp_loadField.
+      wp_storeField.
+      wp_loadField.
+      wp_storeField.
+      wp_storeField.
+      wp_loadField.
+      admit. (* TODO: use protocol lemma *)
+    }
+  }
+  { (* case: s.epoch > args.epoch *)
+    wp_storeField.
+    wp_loadField.
+    wp_apply (release_spec with "[-HΦ HΨ Hreply]").
+    {
+      iFrame "HmuInv Hlocked".
+      iNext.
+      iExists _, _, _, _, _, _.
+      iFrame "∗#%".
+    }
+    wp_pures.
+    iNamed "HΨ".
+    iRight in "HΨ".
+    iModIntro.
+    iApply ("HΦ" with "[HΨ]").
+    2:{
+      instantiate (1:=applyAsFollowerReply.mkC _).
+      iFrame.
+    }
+    {
+      iApply "HΨ".
+      done.
+    }
+  }
+Admitted.
+
+End applyasfollower_proof.
